theories/Classes/Morphisms_Prop.v
@@ -1,0 +1,123 @@
+(************************************************************************)
+(*         *   The Coq Proof Assistant / The Coq Development Team       *)
+(*  v      *         Copyright INRIA, CNRS and contributors             *)
+(* <O___,, * (see version control and CREDITS file for authors & dates) *)
+(*   \VV/  **************************************************************)
+(*    //   *    This file is distributed under the terms of the         *)
+(*         *     GNU Lesser General Public License Version 2.1          *)
+(*         *     (see LICENSE file for the text of the license)         *)
+(************************************************************************)
+
+(** * [Proper] instances for propositional connectives.
+
+   Author: Matthieu Sozeau
+   Institution: LRI, CNRS UMR 8623 - University Paris Sud
+*)
+
+Require Import Coq.Classes.Morphisms.
+Require Import Coq.Program.Basics.
+Require Import Coq.Program.Tactics.
+
+Local Obligation Tactic := try solve [simpl_relation | firstorder auto].
+
+(** Standard instances for [not], [iff] and [impl]. *)
+
+(** Logical negation. *)
+
+#[global]
+Program Instance not_impl_morphism@{s|?|?} :
+  Proper (arrow --> arrow) not@{s|_} | 1.
+
+Print not_impl_morphism.
+
+#[global]
+Program Instance not_iff_morphism@{s|?|} :
+  Proper (iff ++> iff) not@{s|_}.
+
+(** Logical conjunction. *)
+
+#[global]
+Program Instance and_impl_morphism@{s|?|} :
+  Proper (arrow ==> arrow ==> arrow) prod@{s|_ _} | 1.
+
+#[global]
+Program Instance and_iff_morphism@{s|?|} :
+  Proper (iff ==> iff ==> iff) prod@{s|_ _}.
+
+(** Logical implication [impl] is a morphism for logical equivalence. *)
+
+#[global]
+Program Instance iff_iff_iff_impl_morphism@{s s'|?|} : Proper (iff ==> iff ==> iff) arrow@{s s'|_ _}.
+
+(** Morphisms for quantifiers *)
+
+About pointwise_relation.
+
+#[global]
+Program Instance ex_iff_morphism@{s s' s''|?|} {A : Type@{s|_}} : Proper (pointwise_relation@{s Type s'|_ _ _} A iff@{s'|_ _} ==> iff) (@sigma@{s s' s''|_ _} A).
+Next Obligation.
+hnf.
+intros x y [] ? ? ?.
+constructor.
+- firstorder.
+- firstorder. exact (snd fst0).
+Qed.
+
+#[global]
+Program Instance ex_flip_impl_morphism@{s|?|?} {A : Type@{s|_}} :
+  Proper (pointwise_relation A (flip arrow) ==> flip arrow) (@sigmaR@{s|_ _} A) | 1.
+
+#[global]
+Program Instance all_iff_morphism@{s s'|?|} {A : Type@{s|_}} :
+  Proper (pointwise_relation A iff ==> iff) (@all@{s s'|_ _} A).
+Next Obligation.
+intros A x y r.
+constructor; intros H a;  apply r, H.
+Qed.
+
+#[global]
+Program Instance all_impl_morphism {A : Type} :
+  Proper (pointwise_relation A impl ==> impl) (@all A) | 1.
+
+#[global]
+Program Instance all_flip_impl_morphism {A : Type} :
+  Proper (pointwise_relation A (flip impl) ==> flip impl) (@all A) | 1.
+
+(** Equivalent points are simultaneously accessible or not *)
+
+#[global]
+Instance Acc_pt_morphism {A:Type}(E R : A->A->Prop)
+ `(Equivalence _ E) `(Proper _ (E==>E==>iff) R) :
+ Proper (E==>iff) (Acc R).
+Proof.
+  apply proper_sym_arrow_iff.
+  - auto with relations.
+  - intros x y EQ WF. apply Acc_intro; intros z Hz. assert (R z x). specialize (H0 z z (reflexivity _) _ _ EQ). destruct H0. eauto.
+    apply Acc_inv with x; assumption.
+Qed.
+
+(** Equivalent relations have the same accessible points *)
+
+#[global]
+Instance Acc_rel_morphism {A:Type} :
+ @Proper@{Type Prop|_ _} ((A -> A -> Prop) -> A -> Prop) (relation_equivalence ==> eq ==> iff@{Prop|_ _}) (@Acc A).
+Proof.
+  apply proper_sym_arrow_iff_2.
+  - red. symmetry. assumption.
+  - red. symmetry. assumption.
+  - intros R R' EQ a a' Ha WF. subst a.
+    induction WF as [x _ WF']. constructor.
+    intros y Ryx. apply WF', EQ. assumption.
+Qed.
+
+About Acc_rel_morphism.
+
+(** Equivalent relations are simultaneously well-founded or not *)
+
+#[global]
+Instance well_founded_morphism {A : Type} :
+ Proper@{Type Prop|_ _} (relation_equivalence ==> iff) (@well_founded A).
+Proof.
+ unfold well_founded. intros x y r.
+ constructor; intros H a. rewrite <- r. hnf. solve_proper.
+Qed.
